examples/containers/lib/intset-properties.v
@@ -1,0 +1,447 @@
+(* Default settings (from HsToCoq.Coq.Preamble) *)
+
+Generalizable All Variables.
+
+Unset Implicit Arguments.
+Set Maximal Implicit Insertion.
+Unset Strict Implicit.
+Unset Printing Implicit Defensive.
+
+Require Coq.Program.Tactics.
+Require Coq.Program.Wf.
+
+(* Preamble *)
+
+From mathcomp Require Import ssreflect ssrbool.
+Set Bullet Behavior "Strict Subproofs".
+
+Require Coq.ZArith.BinInt.
+Local Notation Zpow := Coq.ZArith.BinInt.Z.pow.
+Local Notation Zle  := Coq.ZArith.BinInt.Z.le.
+
+Require GHC.Enum.
+Notation enumFromTo := GHC.Enum.enumFromTo.
+
+Require GHC.Base.
+Import GHC.Base.Notations.
+
+Require GHC.Num.
+
+Require IntSetProofs.
+
+Record Gen a := MkGen { unGen : a -> Prop }.
+Arguments MkGen {_} _.
+Arguments unGen {_} _ _.
+
+Class Arbitrary (a : Type) := { arbitrary : Gen a }.
+
+Class Propable (a : Type) := { toProp : a -> Prop }.
+
+
+Definition forAll {a prop} `{Propable prop} (g : Gen a) (p : a -> prop) : Prop :=
+  forall (x : a), unGen g x -> toProp (p x).
+
+
+Instance Propable_Prop : Propable Prop :=
+  { toProp := id }.
+
+Instance Propable_bool : Propable bool :=
+  { toProp := is_true }.
+
+Instance Propable_unit : Propable unit :=
+  { toProp := fun _ => True }.
+
+Instance Propable_fn {a prop} `{Arbitrary a} `{Propable prop} : Propable (a -> prop) :=
+  { toProp := forAll arbitrary }.
+
+
+Definition implies {prop} `{Propable prop} (c : bool) (p : prop) : Prop :=
+  if c then toProp p else True.
+Infix ".==>." := implies (at level 99).
+
+Definition andp {prop1 prop2} `{Propable prop1} `{Propable prop2} (p1 : prop1) (p2 : prop2) : Prop :=
+  toProp p1 /\ toProp p2.
+Infix ".&&." := andp (at level 99).
+
+Definition orp {prop1 prop2} `{Propable prop1} `{Propable prop2} (p1 : prop1) (p2 : prop2) : Prop :=
+  toProp p1 \/ toProp p2.
+Infix ".||." := orp (at level 99).
+
+
+Definition choose {a} `{GHC.Base.Ord a} (range : a * a) : Gen a :=
+  MkGen (fun x => (fst range GHC.Base.<= x) && (x GHC.Base.<= snd range)).
+
+
+Definition skip_classify {prop} `{Propable prop} (_ : bool) (_ : GHC.Base.String) : prop -> Prop :=
+  toProp.
+
+
+Instance Arbitrary_bool : Arbitrary bool :=
+  { arbitrary := MkGen xpredT }.
+
+Instance Arbitrary_Int : Arbitrary GHC.Num.Int :=
+  { arbitrary := MkGen (fun x => Zle 0 x) }. (* For IntSet *)
+
+Instance Arbitrary_list {a} `{Arbitrary a} : Arbitrary (list a) :=
+  { arbitrary := MkGen (Coq.Lists.List.Forall (unGen arbitrary)) }.
+
+Instance Arbitrary_IntSet : Arbitrary Data.IntSet.Internal.IntSet :=
+  { arbitrary := MkGen IntSetProofs.WF }.
+
+(* Converted imports: *)
+
+Require Coq.Lists.List.
+Require Data.Bits.
+Require Data.Foldable.
+Require Data.IntSet.Internal.
+Require Data.OldList.
+Require Data.Set.Internal.
+Require GHC.Base.
+Require GHC.List.
+Require GHC.Num.
+Require GHC.Real.
+Require IntSetValidity.
+Import Data.Bits.Notations.
+Import Data.OldList.Notations.
+Import GHC.Base.Notations.
+Import GHC.Num.Notations.
+
+(* No type declarations to convert. *)
+(* Converted value declarations: *)
+
+(* Translating `instance Test.QuickCheck.Arbitrary.Arbitrary
+   Data.IntSet.Internal.IntSet' failed: OOPS! Cannot find information for class
+   Qualified "Test.QuickCheck.Arbitrary" "Arbitrary" unsupported *)
+
+Definition forValid {a} `{Propable a}
+    : (Data.IntSet.Internal.IntSet -> a) -> Prop :=
+  fun f =>
+    forAll arbitrary GHC.Base.$ (fun t =>
+      skip_classify (Data.IntSet.Internal.size t GHC.Base.== GHC.Num.fromInteger 0)
+      (GHC.Base.hs_string__ "empty") GHC.Base.$ (skip_classify (andb
+                                                               (Data.IntSet.Internal.size t GHC.Base.>
+                                                               GHC.Num.fromInteger 0) (Data.IntSet.Internal.size t
+                                                               GHC.Base.<= GHC.Num.fromInteger 10))
+      (GHC.Base.hs_string__ "small") GHC.Base.$ (skip_classify (andb
+                                                               (Data.IntSet.Internal.size t GHC.Base.>
+                                                               GHC.Num.fromInteger 10) (Data.IntSet.Internal.size t
+                                                               GHC.Base.<= GHC.Num.fromInteger 64))
+      (GHC.Base.hs_string__ "medium") GHC.Base.$ (skip_classify
+      (Data.IntSet.Internal.size t GHC.Base.> GHC.Num.fromInteger 64)
+      (GHC.Base.hs_string__ "large") GHC.Base.$ f t)))).
+
+Definition forValidUnitTree {a} `{Propable a}
+    : (Data.IntSet.Internal.IntSet -> a) -> Prop :=
+  fun f => forValid f.
+
+Definition prop_Valid : Prop :=
+  forValidUnitTree GHC.Base.$ (fun t => IntSetValidity.valid t).
+
+Definition powersOf2 : Data.IntSet.Internal.IntSet :=
+  Data.IntSet.Internal.fromList (Coq.Lists.List.flat_map (fun i =>
+                                                           cons (Zpow (GHC.Num.fromInteger 2) i) nil) (enumFromTo
+                                                         (GHC.Num.fromInteger 0) (GHC.Num.fromInteger 63))).
+
+Definition prop_MaskPow2 : Data.IntSet.Internal.IntSet -> bool :=
+  fix prop_MaskPow2 arg_0__
+        := match arg_0__ with
+             | Data.IntSet.Internal.Bin _ msk left_ right_ => andb
+                                                              (Data.IntSet.Internal.member msk powersOf2) (andb
+                                                              (prop_MaskPow2 left_) (prop_MaskPow2 right_))
+             | _ => true
+           end.
+
+Definition prop_AscDescList : list GHC.Num.Int -> bool :=
+  fun xs =>
+    let s := Data.IntSet.Internal.fromList xs in
+    Data.IntSet.Internal.toAscList s GHC.Base.== GHC.List.reverse
+    (Data.IntSet.Internal.toDescList s).
+
+Definition prop_DescList : list GHC.Num.Int -> bool :=
+  fun xs =>
+    (GHC.List.reverse (Data.OldList.sort (Data.OldList.nub xs)) GHC.Base.==
+    Data.IntSet.Internal.toDescList (Data.IntSet.Internal.fromList xs)).
+
+Definition prop_Diff : list GHC.Num.Int -> list GHC.Num.Int -> Prop :=
+  fun xs ys =>
+    match Data.IntSet.Internal.difference (Data.IntSet.Internal.fromList xs)
+            (Data.IntSet.Internal.fromList ys) with
+      | t => IntSetValidity.valid t .&&.(**) (Data.IntSet.Internal.toAscList t
+             GHC.Base.== Data.OldList.sort (_Data.OldList.\\_ (Data.OldList.nub xs)
+                                           (Data.OldList.nub ys)))
+    end.
+
+Definition prop_EmptyValid : Prop :=
+  IntSetValidity.valid Data.IntSet.Internal.empty.
+
+Definition prop_InsertDelete
+    : GHC.Num.Int -> Data.IntSet.Internal.IntSet -> Prop :=
+  fun k t =>
+    negb (Data.IntSet.Internal.member k t) .==>.(**)
+    (match Data.IntSet.Internal.delete k (Data.IntSet.Internal.insert k t) with
+      | t' => IntSetValidity.valid t' .&&.(**) (t' GHC.Base.== t)
+    end).
+
+Definition prop_InsertIntoEmptyValid : GHC.Num.Int -> Prop :=
+  fun x =>
+    IntSetValidity.valid (Data.IntSet.Internal.insert x Data.IntSet.Internal.empty).
+
+Definition prop_Int : list GHC.Num.Int -> list GHC.Num.Int -> Prop :=
+  fun xs ys =>
+    match Data.IntSet.Internal.intersection (Data.IntSet.Internal.fromList xs)
+            (Data.IntSet.Internal.fromList ys) with
+      | t => IntSetValidity.valid t .&&.(**) (Data.IntSet.Internal.toAscList t
+             GHC.Base.== Data.OldList.sort (Data.OldList.nub ((Data.OldList.intersect) (xs)
+                                                             (ys))))
+    end.
+
+Definition prop_LeftRight : Data.IntSet.Internal.IntSet -> bool :=
+  fun arg_0__ =>
+    match arg_0__ with
+      | Data.IntSet.Internal.Bin _ msk left_ right_ => andb (Data.Foldable.and
+                                                            (Coq.Lists.List.flat_map (fun x =>
+                                                                                       cons ((x Data.Bits..&.(**) msk)
+                                                                                            GHC.Base.==
+                                                                                            GHC.Num.fromInteger 0) nil)
+                                                                                     (Data.IntSet.Internal.toList
+                                                                                     left_))) (Data.Foldable.and
+                                                            (Coq.Lists.List.flat_map (fun x =>
+                                                                                       cons ((x Data.Bits..&.(**) msk)
+                                                                                            GHC.Base.== msk) nil)
+                                                                                     (Data.IntSet.Internal.toList
+                                                                                     right_)))
+      | _ => true
+    end.
+
+Definition prop_List : list GHC.Num.Int -> bool :=
+  fun xs =>
+    (Data.OldList.sort (Data.OldList.nub xs) GHC.Base.==
+    Data.IntSet.Internal.toAscList (Data.IntSet.Internal.fromList xs)).
+
+Definition prop_Member : list GHC.Num.Int -> GHC.Num.Int -> bool :=
+  fun xs n =>
+    let m := Data.IntSet.Internal.fromList xs in
+    Data.Foldable.all (fun k =>
+                        Data.IntSet.Internal.member k m GHC.Base.== (Data.Foldable.elem k xs)) (cons n
+                                                                                                     xs).
+
+Definition prop_MemberFromList : list GHC.Num.Int -> bool :=
+  fun xs =>
+    let abs_xs :=
+      Coq.Lists.List.flat_map (fun x =>
+                                if x GHC.Base./= GHC.Num.fromInteger 0 : bool
+                                then cons (GHC.Num.abs x) nil
+                                else nil) xs in
+    let t := Data.IntSet.Internal.fromList abs_xs in
+    andb (Data.Foldable.all (fun arg_2__ => Data.IntSet.Internal.member arg_2__ t)
+         abs_xs) (Data.Foldable.all ((fun arg_3__ =>
+                                      Data.IntSet.Internal.notMember arg_3__ t) GHC.Base.∘ GHC.Num.negate) abs_xs).
+
+Definition prop_NotMember : list GHC.Num.Int -> GHC.Num.Int -> bool :=
+  fun xs n =>
+    let m := Data.IntSet.Internal.fromList xs in
+    Data.Foldable.all (fun k =>
+                        Data.IntSet.Internal.notMember k m GHC.Base.== (Data.Foldable.notElem k xs))
+    (cons n xs).
+
+Definition prop_Prefix : Data.IntSet.Internal.IntSet -> bool :=
+  fix prop_Prefix arg_0__
+        := match arg_0__ with
+             | (Data.IntSet.Internal.Bin prefix msk left_ right_ as s) => andb
+                                                                          (Data.Foldable.all (fun elem =>
+                                                                                               Data.IntSet.Internal.match_
+                                                                                               elem prefix msk)
+                                                                          (Data.IntSet.Internal.toList s)) (andb
+                                                                          (prop_Prefix left_) (prop_Prefix right_))
+             | _ => true
+           end.
+
+Definition prop_Single : GHC.Num.Int -> bool :=
+  fun x =>
+    (Data.IntSet.Internal.insert x Data.IntSet.Internal.empty GHC.Base.==
+    Data.IntSet.Internal.singleton x).
+
+Definition prop_SingletonValid : GHC.Num.Int -> Prop :=
+  fun x => IntSetValidity.valid (Data.IntSet.Internal.singleton x).
+
+Definition prop_UnionAssoc
+    : Data.IntSet.Internal.IntSet -> Data.IntSet.Internal.IntSet -> Data.IntSet.Internal.IntSet -> bool :=
+  fun t1 t2 t3 =>
+    Data.IntSet.Internal.union t1 (Data.IntSet.Internal.union t2 t3) GHC.Base.==
+    Data.IntSet.Internal.union (Data.IntSet.Internal.union t1 t2) t3.
+
+Definition prop_UnionComm
+    : Data.IntSet.Internal.IntSet -> Data.IntSet.Internal.IntSet -> bool :=
+  fun t1 t2 =>
+    (Data.IntSet.Internal.union t1 t2 GHC.Base.== Data.IntSet.Internal.union t2 t1).
+
+Definition prop_UnionInsert
+    : GHC.Num.Int -> Data.IntSet.Internal.IntSet -> Prop :=
+  fun x t =>
+    match Data.IntSet.Internal.union t (Data.IntSet.Internal.singleton x) with
+      | t' => IntSetValidity.valid t' .&&.(**) (t' GHC.Base.==
+              Data.IntSet.Internal.insert x t)
+    end.
+
+Definition prop_disjoint
+    : Data.IntSet.Internal.IntSet -> Data.IntSet.Internal.IntSet -> bool :=
+  fun a b =>
+    Data.IntSet.Internal.disjoint a b GHC.Base.== Data.IntSet.Internal.null
+    (Data.IntSet.Internal.intersection a b).
+
+Definition prop_filter : Data.IntSet.Internal.IntSet -> GHC.Num.Int -> Prop :=
+  fun s i =>
+    let evens := Data.IntSet.Internal.filter GHC.Real.even s in
+    let odds := Data.IntSet.Internal.filter GHC.Real.odd s in
+    let parts := Data.IntSet.Internal.partition GHC.Real.odd s in
+    IntSetValidity.valid odds .&&.(**) (IntSetValidity.valid evens .&&.(**) (parts
+    GHC.Base.== pair odds evens)).
+
+Definition prop_foldL : Data.IntSet.Internal.IntSet -> bool :=
+  fun s =>
+    Data.IntSet.Internal.foldl (GHC.Base.flip cons) nil s GHC.Base.==
+    Data.Foldable.foldl (GHC.Base.flip cons) nil (Data.IntSet.Internal.toList s).
+
+Definition prop_foldL' : Data.IntSet.Internal.IntSet -> bool :=
+  fun s =>
+    Data.IntSet.Internal.foldl' (GHC.Base.flip cons) nil s GHC.Base.==
+    Data.Foldable.foldl' (GHC.Base.flip cons) nil (Data.IntSet.Internal.toList s).
+
+Definition prop_foldR : Data.IntSet.Internal.IntSet -> bool :=
+  fun s =>
+    Data.IntSet.Internal.foldr cons nil s GHC.Base.== Data.IntSet.Internal.toList s.
+
+Definition prop_foldR' : Data.IntSet.Internal.IntSet -> bool :=
+  fun s =>
+    Data.IntSet.Internal.foldr' cons nil s GHC.Base.== Data.IntSet.Internal.toList
+    s.
+
+Definition prop_isProperSubsetOf2
+    : Data.IntSet.Internal.IntSet -> Data.IntSet.Internal.IntSet -> bool :=
+  fun a b =>
+    let c := Data.IntSet.Internal.union a b in
+    Data.IntSet.Internal.isProperSubsetOf a c GHC.Base.== (a GHC.Base./= c).
+
+Definition prop_isSubsetOf2
+    : Data.IntSet.Internal.IntSet -> Data.IntSet.Internal.IntSet -> bool :=
+  fun a b => Data.IntSet.Internal.isSubsetOf a (Data.IntSet.Internal.union a b).
+
+Definition prop_map : Data.IntSet.Internal.IntSet -> bool :=
+  fun s => Data.IntSet.Internal.map GHC.Base.id s GHC.Base.== s.
+
+Definition prop_ord
+    : Data.IntSet.Internal.IntSet -> Data.IntSet.Internal.IntSet -> bool :=
+  fun s1 s2 =>
+    GHC.Base.compare s1 s2 GHC.Base.== GHC.Base.compare (Data.IntSet.Internal.toList
+                                                        s1) (Data.IntSet.Internal.toList s2).
+
+Definition prop_partition
+    : Data.IntSet.Internal.IntSet -> GHC.Num.Int -> Prop :=
+  fun s i =>
+    match Data.IntSet.Internal.partition GHC.Real.odd s with
+      | pair s1 s2 => IntSetValidity.valid s1 .&&.(**) (IntSetValidity.valid s2
+                      .&&.(**) (Data.Foldable.all GHC.Real.odd (Data.IntSet.Internal.toList s1)
+                      .&&.(**) (Data.Foldable.all GHC.Real.even (Data.IntSet.Internal.toList s2)
+                      .&&.(**) (s GHC.Base.== Data.IntSet.Internal.union s1 s2))))
+    end.
+
+Definition prop_size : Data.IntSet.Internal.IntSet -> Prop :=
+  fun s =>
+    let sz := Data.IntSet.Internal.size s in
+    (sz GHC.Base.== Data.IntSet.Internal.foldl' (fun arg_1__ arg_2__ =>
+                                                  match arg_1__ , arg_2__ with
+                                                    | i , _ => i GHC.Num.+ GHC.Num.fromInteger 1
+                                                  end) (GHC.Num.fromInteger 0 : GHC.Num.Int) s) .&&.(**) (sz GHC.Base.==
+    Data.Foldable.length (Data.IntSet.Internal.toList s)).
+
+Definition prop_split : Data.IntSet.Internal.IntSet -> GHC.Num.Int -> Prop :=
+  fun s i =>
+    match Data.IntSet.Internal.split i s with
+      | pair s1 s2 => IntSetValidity.valid s1 .&&.(**) (IntSetValidity.valid s2
+                      .&&.(**) (Data.Foldable.all (fun arg_1__ => arg_1__ GHC.Base.< i)
+                      (Data.IntSet.Internal.toList s1) .&&.(**) (Data.Foldable.all (fun arg_2__ =>
+                                                                                     arg_2__ GHC.Base.> i)
+                      (Data.IntSet.Internal.toList s2) .&&.(**) (Data.IntSet.Internal.delete i s
+                      GHC.Base.== Data.IntSet.Internal.union s1 s2))))
+    end.
+
+Definition prop_splitMember
+    : Data.IntSet.Internal.IntSet -> GHC.Num.Int -> Prop :=
+  fun s i =>
+    match Data.IntSet.Internal.splitMember i s with
+      | pair (pair s1 t) s2 => IntSetValidity.valid s1 .&&.(**) (IntSetValidity.valid
+                               s2 .&&.(**) (Data.Foldable.all (fun arg_1__ => arg_1__ GHC.Base.< i)
+                               (Data.IntSet.Internal.toList s1) .&&.(**) (Data.Foldable.all (fun arg_2__ =>
+                                                                                              arg_2__ GHC.Base.> i)
+                               (Data.IntSet.Internal.toList s2) .&&.(**) ((t GHC.Base.==
+                               Data.IntSet.Internal.member i s) .&&.(**) (Data.IntSet.Internal.delete i s
+                               GHC.Base.== Data.IntSet.Internal.union s1 s2)))))
+    end.
+
+Definition prop_splitRoot : Data.IntSet.Internal.IntSet -> bool :=
+  fun s =>
+    let loop :=
+      fun arg_0__ =>
+        match arg_0__ with
+          | nil => true
+          | cons s1 rst => Data.Foldable.null (Coq.Lists.List.flat_map (fun x =>
+                                                                         Coq.Lists.List.flat_map (fun y =>
+                                                                                                   if x GHC.Base.>
+                                                                                                      y : bool
+                                                                                                   then cons (pair x y)
+                                                                                                             nil
+                                                                                                   else nil)
+                                                                                                 (Data.IntSet.Internal.toList
+                                                                                                 (Data.IntSet.Internal.unions
+                                                                                                 rst)))
+                                                                       (Data.IntSet.Internal.toList s1))
+        end in
+    let ls := Data.IntSet.Internal.splitRoot s in
+    andb (loop ls) (s GHC.Base.== Data.IntSet.Internal.unions ls).
+
+Definition toSet : Data.IntSet.Internal.IntSet -> Data.Set.Internal.Set_
+                   GHC.Num.Int :=
+  Data.Set.Internal.fromList GHC.Base.∘ Data.IntSet.Internal.toList.
+
+Definition prop_isSubsetOf
+    : Data.IntSet.Internal.IntSet -> Data.IntSet.Internal.IntSet -> bool :=
+  fun a b =>
+    Data.IntSet.Internal.isSubsetOf a b GHC.Base.== Data.Set.Internal.isSubsetOf
+    (toSet a) (toSet b).
+
+Definition prop_isProperSubsetOf
+    : Data.IntSet.Internal.IntSet -> Data.IntSet.Internal.IntSet -> bool :=
+  fun a b =>
+    Data.IntSet.Internal.isProperSubsetOf a b GHC.Base.==
+    Data.Set.Internal.isProperSubsetOf (toSet a) (toSet b).
+
+(* Unbound variables:
+     Prop Propable Zpow andb arbitrary bool cons enumFromTo forAll list negb nil
+     op_zizazazi__ op_zizezezgzi__ pair skip_classify true Coq.Lists.List.flat_map
+     Data.Bits.op_zizazi__ Data.Foldable.all Data.Foldable.and Data.Foldable.elem
+     Data.Foldable.foldl Data.Foldable.foldl' Data.Foldable.length
+     Data.Foldable.notElem Data.Foldable.null Data.IntSet.Internal.Bin
+     Data.IntSet.Internal.IntSet Data.IntSet.Internal.delete
+     Data.IntSet.Internal.difference Data.IntSet.Internal.disjoint
+     Data.IntSet.Internal.empty Data.IntSet.Internal.filter
+     Data.IntSet.Internal.foldl Data.IntSet.Internal.foldl'
+     Data.IntSet.Internal.foldr Data.IntSet.Internal.foldr'
+     Data.IntSet.Internal.fromList Data.IntSet.Internal.insert
+     Data.IntSet.Internal.intersection Data.IntSet.Internal.isProperSubsetOf
+     Data.IntSet.Internal.isSubsetOf Data.IntSet.Internal.map
+     Data.IntSet.Internal.match_ Data.IntSet.Internal.member
+     Data.IntSet.Internal.notMember Data.IntSet.Internal.null
+     Data.IntSet.Internal.partition Data.IntSet.Internal.singleton
+     Data.IntSet.Internal.size Data.IntSet.Internal.split
+     Data.IntSet.Internal.splitMember Data.IntSet.Internal.splitRoot
+     Data.IntSet.Internal.toAscList Data.IntSet.Internal.toDescList
+     Data.IntSet.Internal.toList Data.IntSet.Internal.union
+     Data.IntSet.Internal.unions Data.OldList.intersect Data.OldList.nub
+     Data.OldList.op_zrzr__ Data.OldList.sort Data.Set.Internal.Set_
+     Data.Set.Internal.fromList Data.Set.Internal.isProperSubsetOf
+     Data.Set.Internal.isSubsetOf GHC.Base.compare GHC.Base.flip GHC.Base.id
+     GHC.Base.op_z2218U__ GHC.Base.op_zd__ GHC.Base.op_zeze__ GHC.Base.op_zg__
+     GHC.Base.op_zl__ GHC.Base.op_zlze__ GHC.Base.op_zsze__ GHC.List.reverse
+     GHC.Num.Int GHC.Num.abs GHC.Num.negate GHC.Num.op_zp__ GHC.Real.even
+     GHC.Real.odd IntSetValidity.valid
+*)
