examples/containers/module-edits/intset-properties/preamble.v
@@ -1,0 +1,75 @@
+From mathcomp Require Import ssreflect ssrbool.
+Set Bullet Behavior "Strict Subproofs".
+
+Require Coq.ZArith.BinInt.
+Local Notation Zpow := Coq.ZArith.BinInt.Z.pow.
+Local Notation Zle  := Coq.ZArith.BinInt.Z.le.
+
+Require GHC.Enum.
+Notation enumFromTo := GHC.Enum.enumFromTo.
+
+Require GHC.Base.
+Import GHC.Base.Notations.
+
+Require GHC.Num.
+
+Require IntSetProofs.
+
+Record Gen a := MkGen { unGen : a -> Prop }.
+Arguments MkGen {_} _.
+Arguments unGen {_} _ _.
+
+Class Arbitrary (a : Type) := { arbitrary : Gen a }.
+
+Class Propable (a : Type) := { toProp : a -> Prop }.
+
+
+Definition forAll {a prop} `{Propable prop} (g : Gen a) (p : a -> prop) : Prop :=
+  forall (x : a), unGen g x -> toProp (p x).
+
+
+Instance Propable_Prop : Propable Prop :=
+  { toProp := id }.
+
+Instance Propable_bool : Propable bool :=
+  { toProp := is_true }.
+
+Instance Propable_unit : Propable unit :=
+  { toProp := fun _ => True }.
+
+Instance Propable_fn {a prop} `{Arbitrary a} `{Propable prop} : Propable (a -> prop) :=
+  { toProp := forAll arbitrary }.
+
+
+Definition implies {prop} `{Propable prop} (c : bool) (p : prop) : Prop :=
+  if c then toProp p else True.
+Infix ".==>." := implies (at level 99).
+
+Definition andp {prop1 prop2} `{Propable prop1} `{Propable prop2} (p1 : prop1) (p2 : prop2) : Prop :=
+  toProp p1 /\ toProp p2.
+Infix ".&&." := andp (at level 99).
+
+Definition orp {prop1 prop2} `{Propable prop1} `{Propable prop2} (p1 : prop1) (p2 : prop2) : Prop :=
+  toProp p1 \/ toProp p2.
+Infix ".||." := orp (at level 99).
+
+
+Definition choose {a} `{GHC.Base.Ord a} (range : a * a) : Gen a :=
+  MkGen (fun x => (fst range GHC.Base.<= x) && (x GHC.Base.<= snd range)).
+
+
+Definition skip_classify {prop} `{Propable prop} (_ : bool) (_ : GHC.Base.String) : prop -> Prop :=
+  toProp.
+
+
+Instance Arbitrary_bool : Arbitrary bool :=
+  { arbitrary := MkGen xpredT }.
+
+Instance Arbitrary_Int : Arbitrary GHC.Num.Int :=
+  { arbitrary := MkGen (fun x => Zle 0 x) }. (* For IntSet *)
+
+Instance Arbitrary_list {a} `{Arbitrary a} : Arbitrary (list a) :=
+  { arbitrary := MkGen (Coq.Lists.List.Forall (unGen arbitrary)) }.
+
+Instance Arbitrary_IntSet : Arbitrary Data.IntSet.Internal.IntSet :=
+  { arbitrary := MkGen IntSetProofs.WF }.
