examples/containers/proofs/IntSetPropertyProofs.v
@@ -1,0 +1,591 @@
+From mathcomp Require Import ssreflect ssrbool ssrnat ssrfun seq eqtype.
+Set Bullet Behavior "Strict Subproofs".
+
+Require Import GHC.Base      Proofs.GHC.Base.
+Require Import Data.OldList  Proofs.Data.OldList.
+Require Import Data.Foldable Proofs.Data.Foldable.
+Notation list := Coq.Init.Datatypes.list.
+Notation seq  := Coq.Lists.List.seq.
+
+Infix "=="  := op_zeze__ : bool_scope.
+Infix "===" := eq_op (at level 70, no associativity) : bool_scope.
+
+Notation "x == y :> A"  := (op_zeze__ (x : A) (y : A)) : bool_scope.
+Notation "x === y :> A" := (eq_op     (x : A) (y : A)) (at level 70, y at next level, no associativity) : bool_scope.
+
+Notation reflect := ssrbool.reflect. (* Why do I need this? *)
+
+Require Import Sorting.Sorted.
+Notation sort := Data.OldList.sort.
+
+Require Import Data.IntSet.Internal.
+Require Import IntSetProperties.
+Require Import IntSetProofs.
+Module IntSetFSet := Foo.
+
+Arguments "$"          {_ _}     / _ _.
+Arguments id           {_}       / _.
+Arguments Datatypes.id {_}       / _.
+Arguments forAll       {_ _ _ _} / _.
+Arguments "∘"          {_ _}     _ _ _ /.
+
+Theorem thm_Valid : toProp prop_Valid.
+Proof.
+  rewrite /prop_Valid /forValidUnitTree /forValid /=; apply valid_correct.
+Qed.
+
+Lemma WF_Bin_children (p : Prefix) (m : Mask) (l r : IntSet) :
+  WF (Bin p m l r) -> WF l /\ WF r.
+Proof.
+  case=> fn;
+    inversion 1    as [|s bounds fn' desc];
+    subst s fn';
+    inversion desc as [|l' bounds_l fn_l r' bounds_r fn_r
+                        p' m' bounds' fn'
+                        desc_l desc_r is_pos sub_l sub_r def_p def_m spec_fn];
+    subst p' m' l' r' bounds' fn'.
+  split; [exists fn_l | exists fn_r]; eauto using DescSem.
+Qed.
+
+Corollary WF_Bin_left (p : Prefix) (m : Mask) (l r : IntSet) :
+  WF (Bin p m l r) -> WF l.
+Proof. by move=> /WF_Bin_children []. Qed.
+
+Corollary WF_Bin_right (p : Prefix) (m : Mask) (l r : IntSet) :
+  WF (Bin p m l r) -> WF r.
+Proof. by move=> /WF_Bin_children []. Qed.
+
+Fixpoint iterates (n : nat) {a} (f : a -> a) (z : a) : list a :=
+  match n with
+  | O    => nil
+  | S n' => z :: iterates n' f (f z)
+  end.
+
+Lemma eftInt_aux_fuel_case (x y : Int) (p : GHC.Enum.eftInt_aux_fuel x y) :
+  (exists (gt : (x >? y)%Z = true),                  p = @GHC.Enum.done x y gt) \/
+  (exists (p' : GHC.Enum.eftInt_aux_fuel (x+1)%Z y), p = @GHC.Enum.step x y p').
+Proof.
+  case: p => [x' y' gt | x' y' p'].
+  - by left; exists gt.
+  - by right; exists p'.
+Qed.
+
+Require Import Coq.Logic.Eqdep_dec.
+
+Theorem UIP_refl_dec {A : Type} (dec : forall x y : A, {x = y} + {x <> y}) (x : A) (p : x = x) : p = erefl.
+Proof. exact (UIP_dec dec p erefl). Qed.
+
+Require Import GHC.Num.
+
+Theorem eftInt_aux_iterates (from to : Int) p :
+  @GHC.Enum.eftInt_aux from to p = iterates (Z.to_nat (to - from + #1)) (fun x => x + #1) from.
+Proof.
+  move: to p.
+  elim: from => [| from IHfrom | from IHfrom].
+  - elim=> [| to IHto | to IHto].
+    + move=> p; move: (eftInt_aux_fuel_case _ _ p) => [[gt def_p] | [p' def_p]]; subst p.
+      * by contradict gt.
+      * admit.
+    + simpl.
+Admitted.
+
+Require Import GHC.Num.
+Theorem enumFromTo_Int_iterates (from to : Int) :
+  enumFromTo from to = iterates (Z.to_nat (to - from + #1)) (fun x => x + #1) from.
+Proof. apply eftInt_aux_iterates. Qed.
+
+Theorem thm_MaskPow2 : toProp prop_MaskPow2.
+Proof.
+  simpl; elim=> [p m l IHl r IHr | p m | ] WF_s //=.
+  apply/and3P; split.
+  - rewrite /powersOf2 enumFromTo_Int_iterates.
+    cbv -[Z.pow member fromList].
+
+    inversion WF_s; inversion H; inversion HD; subst.
+    rewrite /rMask.
+    destruct r0 as [r0_1 r0_2].
+    
+(*     rewrite /powersOf2 enumFromTo_Int_iterates. *)
+(*     cbv -[Zpow member fromList]. *)
+
+    
+(*     move: (WF_s) => /WF_Bin_children [/IHl Pl /IHr Pr]. *)
+(*     move: Pl Pr; rewrite /prop_MaskPow2. *)
+
+(* rewrite /powersOf2 enumFromTo_Int_iterates. *)
+(*     cbv -[Zpow member fromList]. *)
+    
+(*     simpl *)
+
+(*  /=. *)
+(*     replace (GHC.Enum.eftInt 0%Z 63%Z) with (eftInt 0%Z 63%Z) by admit. *)
+    
+
+(*     cbv -[member fromList flat_map Zpow]. *)
+
+(*     rewrite /Enum.eftInt_fuel. *)
+    
+(*   - apply IHl; move: WF_s; apply WF_Bin_left. *)
+(*   - apply IHr; move: WF_s; apply WF_Bin_right. *)
+Abort.
+
+Theorem thm_AscDescList : toProp prop_AscDescList.
+Proof.
+  rewrite /prop_AscDescList /= => xs _.
+  rewrite /fromList /foldl /Foldable__list /Data.Foldable.Foldable__list_foldl /foldl /=.
+  rewrite /toAscList /toDescList.
+  rewrite foldl_foldr; last admit.
+  rewrite /flip.
+  unfold "_==_", Eq_list => /=.
+  
+  elim: xs => [|x xs IH] //=.
+Abort.
+
+Theorem thm_DescList : toProp prop_DescList.
+Proof.
+Abort.
+
+Theorem thm_Diff : toProp prop_Diff.
+Proof.
+  rewrite /prop_Diff /= => xs POS_xs ys POS_ys.
+  
+  move: (fromList_WF   xs POS_xs)       => WF_xs.
+  move: (fromList_WF   ys POS_ys)       => WF_ys.
+  move: (difference_WF _ _ WF_xs WF_ys) => WF_diff.
+  
+  split=> /=; first by apply valid_correct.
+Abort.
+
+Theorem thm_EmptyValid : toProp prop_EmptyValid.
+Proof. done. Qed.
+
+Lemma WRONG : forall x : Z, exists x' : N, x = Z.of_N x'. Admitted.
+Lemma eqIntSetMemberP {s1 s2 : IntSet} :
+  WF s1 -> WF s2 ->
+  reflect (forall x, member x s1 == member x s2) (s1 == s2).
+Proof.
+  move=> WF1 WF2.
+  set s1' := exist _ _ WF1; set s2' := exist _ _ WF2.
+  move: (IntSetFSet.equal_1 s1' s2') (IntSetFSet.equal_2 s1' s2').
+  rewrite /= /IntSetFSet.Equal /= /IntSetFSet.In_set => Equal_eq eq_Equal.
+  apply iff_reflect; split.
+  - move=> KEYS; apply Equal_eq=> n; apply eq_iff_eq_true.
+    move: KEYS; cbv -[member Z.of_N eqb is_true].
+    rewrite -eqb_true_iff; apply.
+  - move=> /eq_Equal KEYS x; move: (WRONG x) => [n def_x]; subst x.
+    move: (KEYS n); cbv -[member Z.of_N eqb iff].
+    case: (member _ s1); case: (member _ s2); tauto.
+Qed.
+
+Theorem Sem_member (s : IntSet) :
+  WF s ->
+  Sem s (member ^~ s).
+Proof.
+  move=> [f def_f].
+  apply Sem_change_f with f => //.
+  by move: (def_f) => /member_Sem.
+Qed.
+
+Ltac member_by_Sem SEM :=
+  repeat (move=> /Sem_member ? || move=> ?);
+  erewrite member_Sem;
+    last (eapply SEM; try eassumption; reflexivity);
+    reflexivity.
+
+Lemma insert_member (x : Int) (s : IntSet) :
+  (0 <= x)%Z -> WF s ->
+  forall k, member k (insert x s) = (k == x) || member k s.
+Proof. member_by_Sem insert_Sem. Qed.
+
+Lemma delete_member (x : Int) (s : IntSet) :
+  (0 <= x)%Z -> WF s ->
+  forall k, member k (delete x s) = (k /= x) && member k s.
+Proof. member_by_Sem delete_Sem. Qed.
+
+Lemma union_member (s1 s2 : IntSet) :
+  WF s1 -> WF s2 ->
+  forall k, member k (union s1 s2) = member k s1 || member k s2.
+Proof. member_by_Sem union_Sem. Qed.
+
+Lemma intersection_member (s1 s2 : IntSet) :
+  WF s1 -> WF s2 ->
+  forall k, member k (intersection s1 s2) = member k s1 && member k s2.
+Proof. member_by_Sem intersection_Sem. Qed.
+
+Lemma difference_member (s1 s2 : IntSet) :
+  WF s1 -> WF s2 ->
+  forall k, member k (difference s1 s2) = member k s1 && ~~ member k s2.
+Proof. member_by_Sem difference_Sem. Qed.
+
+Lemma singleton_member (x : Int) :
+  (0 <= x)%Z ->
+  forall k, member k (singleton x) = (k == x).
+Proof. member_by_Sem singleton_Sem. Qed.
+
+Lemma EqExact_cases {A} `{EqExact A} (x y : A) :
+  {x == y /\ x = y} + {x /= y /\ x <> y}.
+Proof.
+  rewrite Neq_inv; case CMP: (x == y).
+  - by left; split=> //; apply/Eq_eq.
+  - by right; split=> //; move=> /Eq_eq; rewrite CMP.
+Qed.
+
+Theorem thm_InsertDelete : toProp prop_InsertDelete.
+Proof.
+  rewrite /prop_InsertDelete /= => x POS s WF_s.
+
+  move: (insert_WF x _ WF_s   POS) => WF_ins.
+  move: (delete_WF x _ WF_ins POS) => WF_res.
+  case x_nin_s: (~~ member x s) => //=; split=> /=; first by apply valid_correct.
+
+  apply/eqIntSetMemberP => // k; apply/Eq_eq.
+  rewrite delete_member // insert_member //.
+  rewrite Eq_inv andb_orr andbN orFb.
+  
+  case: (EqExact_cases k x) => [[Beq Peq] | [Bneq Pneq]].
+  - by rewrite Peq; move: x_nin_s => /negbTE->; rewrite andbF.
+  - by rewrite Bneq andTb.
+Qed.
+
+Theorem empty_WF : WF empty.
+Proof. by exists xpred0; constructor. Qed.
+Hint Resolve empty_WF.
+
+Theorem thm_InsertIntoEmptyValid : toProp prop_InsertIntoEmptyValid.
+Proof.
+  rewrite /prop_InsertIntoEmptyValid /= => x POS.
+  by apply valid_correct, insert_WF.
+Qed.
+
+Hypothesis sorted_sort : forall {A} `{Ord A} (xs : list A),
+  StronglySorted _<=_ (sort xs).
+
+Theorem elem_by_In {A} `{EqExact A} (xs : list A) (x : A) :
+  reflect (In x xs) (elem_by _==_ x xs).
+Proof.
+  elim: xs => [|x' xs IH] /=; first by constructor.
+  apply iff_reflect; split;
+    try move=> /orP;
+    move=> [? | ?];
+    try apply/orP;
+    solve [by left; apply/Eq_eq | by right; apply/IH].
+Qed.
+
+Hypothesis nub_NoDup : forall {A} `{EqExact A} (xs : list A),
+  NoDup (nub xs).
+
+Theorem thm_Int : toProp prop_Int.
+Proof.
+  rewrite /prop_Int /= => xs POS_xs ys POS_ys.
+
+  move: (fromList_WF     xs POS_xs)       => WF_xs.
+  move: (fromList_WF     ys POS_ys)       => WF_ys.
+  move: (intersection_WF _ _ WF_xs WF_ys) => WF_both.
+
+  split=> /=; first by apply valid_correct.
+  apply/Eq_eq; fold toList.
+Abort.
+
+Lemma Foldable_and_all {F} `{Foldable F} : and (t := F) =1 all id.
+Proof. done. Qed.
+
+Lemma toList_member_has (s : IntSet) :
+  WF s ->
+  forall k, has (_==_ k) (toList s) = member k s.
+Proof.
+  move=> /Sem_member/toList_In SEM k.
+  case CONT: (member k s) (SEM k) => SEM_k.
+  - have: In k (toList s) by apply SEM_k. clear SEM_k.
+    elim: (toList s) => [|x xs IH] //= SEM_k.
+    case: SEM_k => [-> | IN].
+    + by rewrite Eq_refl orTb.
+    + by rewrite IH // orbT.
+  - have: ~ In k (toList s) by move=> /SEM_k. clear SEM_k=> SEM_k.
+    apply negbTE; apply /negP; contradict SEM_k.
+    elim: (toList s) SEM_k => [|x xs IH] //= SEM_k.
+    move: SEM_k => /orP [/Eq_eq -> | H]; [by left | by right; apply IH].
+Qed.
+
+Lemma Int_eqbP : Equality.axiom (_==_ : Int -> Int -> bool).
+Proof. exact Eq_eq. Qed.
+
+Canonical Int_eqMixin := EqMixin Int_eqbP.
+Canonical Int_eqType := Eval hnf in EqType Int Int_eqMixin.
+
+Lemma InP {A : eqType} (x : A) (xs : list A) :
+  reflect (In x xs) (x \in xs).
+Proof.
+  elim: xs => [|y ys IH] //=.
+  - by rewrite seq.in_nil; constructor.
+  - rewrite inE; case CMP: (x === y) => /=.
+    + by constructor; left; apply/eqP; rewrite eq_sym.
+    + apply/equivP; first exact IH.
+      split; first by right.
+      case=> // ?; subst.
+      by move: CMP; rewrite eq_refl.
+Qed.
+
+Lemma elemC {A} `{Eq_ A} (a x : A) (xs : list A) : elem a (x :: xs) = (a == x) || elem a xs.
+Proof. done. Qed.
+
+Lemma elemN {A} `{Eq_ A} (a : A) : elem a [::] = false.
+Proof. done. Qed.
+
+Lemma elemP {A} `{EqExact A} (x : A) (xs : list A) :
+  reflect (In x xs) (elem x xs).
+Proof.
+  elim: xs => [|y ys IH] //=; first by constructor.
+  rewrite elemC; case CMP: (x == y) => /=.
+  - by constructor; left; apply/Eq_eq; rewrite Eq_sym.
+  - apply/equivP; first exact IH.
+    split; first by right.
+    case=> // ?; subst.
+    by move: CMP; rewrite Eq_refl.
+Qed.
+
+Lemma eqType_EqExact {A : eqType} `{EqExact A} (x y : A) : (x === y) = (x == y).
+Proof. by case E: (x === y); case E': (x == y)=> //; move: E E' => /eqP ? /Eq_eq ?. Qed.
+
+Lemma EqExact_eqType {A : eqType} `{EqExact A} (x y : A) : (x == y) = (x === y).
+Proof. by rewrite eqType_EqExact. Qed.
+
+Lemma elem_in {A : eqType} `{EqExact A} (xs : list A) (a : A) :
+  elem a xs = (a \in xs).
+Proof. by elim: xs => [|x xs IH] //=; rewrite inE -IH eqType_EqExact. Qed.
+
+Lemma in_elem {A : eqType} `{EqExact A} (xs : list A) (a : A) :
+  a \in xs = elem a xs.
+Proof. symmetry; apply elem_in. Qed.
+
+Theorem Foldable_all_ssreflect {A} (p : A -> bool) (xs : list A) : all p xs = seq.all p xs.
+Proof. by rewrite Foldable_all_forallb. Qed.
+
+Lemma fromList_member (xs : list Int) :
+  Forall (fun x => 0 <= x)%Z xs ->
+  forall k, member k (fromList xs) = elem k xs.
+Proof.
+  move=> POS_xs k.
+  move: (fromList_Sem xs POS_xs) => [f [SEM DEF]].
+  erewrite member_Sem; last by eapply SEM.
+  move: (DEF k); case: (f k) => DEF_k.
+  all: by symmetry; apply/elemP/DEF_k.
+Qed.
+
+Lemma toList_member (s : IntSet) :
+  WF s ->
+  forall k, elem k (toList s) = member k s.
+Proof.
+  move=> /Sem_member/toList_In SEM k.
+  by case CONT: (member k s) (SEM k) => SEM_k; apply/elemP/SEM_k.
+Qed.
+
+Theorem Sem_Desc0 : forall s f, Sem s f -> exists r, Desc0 s r f.
+Proof.
+  apply Sem_ind => [f false_f | s r f Desc_srf].
+  - by exists (0%Z,0%N); apply Desc0Nil.
+  - by exists r; apply (Desc0NotNil s r f r f); rewrite // isSubrange_refl.
+Qed.
+
+Theorem thm_LeftRight : toProp prop_LeftRight.
+Proof.
+  rewrite /prop_LeftRight /= => -[p m l r | // | // ] WF_x; move: (WF_x) => /WF_Bin_children [WF_l WF_r].
+  rewrite !Foldable_and_all !Foldable_all_ssreflect !flat_map_cons_f;
+    apply/andP; split; apply/allP => /= b /mapP [] x; rewrite in_elem toList_member // => x_in {b}->.
+  - case: (WF_x) => [f /Sem_Desc0 [rng DESC0]].
+    inversion_clear DESC0 as [|s rng' f' rng_ f'_ DESC rng'_rng f_f'].
+    inversion DESC; subst.
+Abort.
+
+Require Import OrdTactic.
+
+Theorem Sort_eq {A : eqType} `{OrdLaws A} `{!EqExact A} (xs ys : list A) :
+  StronglySorted _<=_ xs ->
+  StronglySorted _<=_ ys ->
+  (xs == ys) = seq.all (fun a => a \in xs) ys && seq.all (fun b => b \in ys) xs.
+Proof.
+  elim: xs ys => [|x xs IH_xs] [|y ys] //=.
+  inversion_clear 1 as [|X1 X2 SS_xs FA_xs X3]; inversion_clear 1 as [|X1 X2 SS_ys FA_ys X3].
+  unfold "=="; rewrite /Eq_list /=; case CMP: (x == y).
+  - move: CMP => /Eq_eq ? /=; subst y.
+    replace (eqlist xs ys) with (xs == ys) by done; rewrite IH_xs //.
+    admit.
+  - 
+Admitted.
+
+Theorem thm_List : toProp prop_List.
+Proof.
+  rewrite /prop_List /=; rewrite -/toList => xs POS_xs.
+Abort.
+  
+
+Theorem thm_Member : toProp prop_Member.
+Proof.
+  rewrite /prop_Member /= => xs POS_xs n POS_n.
+  rewrite !Foldable_all_ssreflect; apply/allP => /= k.
+  by rewrite fromList_member // Eq_refl.
+Qed.
+
+Lemma elem_app {A} `{Eq_ A} (a : A) (xs ys : list A) :
+  elem a (xs ++ ys) = elem a xs || elem a ys.
+Proof. by elim: xs => [|x xs] //=; rewrite !elemC -orbA => ->. Qed.
+
+(* Cheating: manually forgetting POS constraint *)
+Theorem thm_MemberFromList : toProp prop_MemberFromList.
+Proof.
+  rewrite /prop_MemberFromList /= => xs _(* POS_xs *).
+  set abs_xs := flat_map _ xs.
+  apply/andP; split.
+  all: rewrite Foldable_all_ssreflect; apply/allP => /= k; rewrite in_elem.
+  - rewrite fromList_member //.
+    subst abs_xs; elim: xs => [|x xs IH] //=.
+    case: (x /= #0) => //=.
+    constructor; last assumption.
+    apply Z.abs_nonneg.
+  - rewrite /notMember /notElem /= fromList_member //.
+    + move=> k_abs; have k_pos: (0 <= k)%Z. {
+        subst abs_xs; elim: xs k_abs => [|x xs IH] //=.
+        rewrite elem_app=> /orP[] //.
+        case NZ: (x /= #0)=> //=.
+        rewrite elemC elemN orbF => /Eq_eq ->.
+        apply Z.abs_nonneg.
+      }
+      clear k_abs; subst abs_xs; elim: xs => [|x xs IH] //=.
+      rewrite elem_app negb_orb IH andbT.
+      by case: k k_pos {IH}; case: x.
+    + apply Forall_forall=> {k} k; rewrite in_flat_map => -[x [_]].
+      case CMP: (x /= #0) => //= -[] //= <-.
+      apply Z.abs_nonneg.
+Qed.      
+
+Theorem thm_NotMember : toProp prop_NotMember.
+Proof.
+  rewrite /prop_NotMember /= => xs POS_xs n POS_n.
+  rewrite !Foldable_all_ssreflect; apply/allP => /= k.
+  by rewrite /notMember /notElem /= fromList_member // Eq_refl.
+Qed.
+
+Theorem thm_Prefix : toProp prop_Prefix.
+Proof.
+Abort.
+
+Theorem thm_Single : toProp prop_Single.
+Proof. by rewrite /prop_Single /= => x POS_x; apply/Eq_eq. Qed.
+
+Theorem thm_SingletonValid : toProp prop_SingletonValid.
+Proof.
+  rewrite /prop_SingletonValid /= => x POS_x.
+  by apply valid_correct, singleton_WF.
+Qed.
+
+Theorem thm_UnionAssoc : toProp prop_UnionAssoc.
+Proof.
+  rewrite /prop_UnionAssoc /= => s1 WF1 s2 WF2 s3 WF3.
+  
+  move: (union_WF _ _ WF1  WF2)  => WF12.
+  move: (union_WF _ _ WF2  WF3)  => WF23.
+  move: (union_WF _ _ WF12 WF3)  => WF123.
+  move: (union_WF _ _ WF1  WF23) => WF123'.
+  
+  apply/eqIntSetMemberP => // k; apply/Eq_eq.
+  by rewrite !union_member // orbA.
+Qed.
+
+Theorem thm_UnionComm : toProp prop_UnionComm.
+Proof.
+Proof.
+  rewrite /prop_UnionComm /= => s1 WF1 s2 WF2.
+  
+  move: (union_WF _ _ WF1 WF2) => WF12.
+  move: (union_WF _ _ WF2 WF1) => WF21.
+  
+  apply/eqIntSetMemberP => // k; apply/Eq_eq.
+  by rewrite !union_member // orbC.
+Qed.
+
+Theorem thm_UnionInsert : toProp prop_UnionInsert.
+Proof.
+  rewrite /prop_UnionInsert /= => x POS_x s WF_s.
+
+  move: (singleton_WF x POS_x)          => WF_sing.
+  move: (union_WF     _ _ WF_s WF_sing) => WF_union.
+  move: (insert_WF    x _ WF_s POS_x)   => WF_ins.
+
+  split=> /=; first by apply valid_correct.
+  
+  apply/eqIntSetMemberP => // k; apply/Eq_eq.
+  by rewrite union_member // singleton_member // insert_member // orbC.
+Qed.
+
+Theorem thm_disjoint : toProp prop_disjoint.
+Proof.
+  rewrite /prop_disjoint /= => s1 WF1 s2 WF2.
+  
+  move: (intersection_WF _ _ WF1 WF2) => WF12.
+  
+  elim: s1 WF1 WF12 => [p m l IHl r IHr | p b | ] WF1 WF12.
+  - 
+Abort.
+
+Theorem thm_filter : toProp prop_filter.
+Proof.
+Abort.
+
+Theorem thm_foldL : toProp prop_foldL.
+Proof.
+Abort.
+
+Theorem thm_foldL : toProp prop_foldL.
+Proof.
+Abort.
+
+Theorem thm_foldR : toProp prop_foldR.
+Proof.
+Abort.
+
+Theorem thm_foldR : toProp prop_foldR.
+Proof.
+Abort.
+
+Theorem thm_isProperSubsetOf : toProp prop_isProperSubsetOf.
+Proof.
+Abort.
+
+Theorem thm_isSubsetOf : toProp prop_isSubsetOf.
+Proof.
+Abort.
+
+Theorem thm_map : toProp prop_map.
+Proof.
+Abort.
+
+Theorem thm_ord : toProp prop_ord.
+Proof.
+Abort.
+
+Theorem thm_partition : toProp prop_partition.
+Proof.
+Abort.
+
+Theorem thm_size : toProp prop_size.
+Proof.
+Abort.
+
+Theorem thm_split : toProp prop_split.
+Proof.
+Abort.
+
+Theorem thm_splitMember : toProp prop_splitMember.
+Proof.
+Abort.
+
+Theorem thm_splitRoot : toProp prop_splitRoot.
+Proof.
+Abort.
+
+Theorem thm_isSubsetOf : toProp prop_isSubsetOf.
+Proof.
+Abort.
+
+Theorem thm_isProperSubsetOf : toProp prop_isProperSubsetOf.
+Proof.
+Abort.
