examples/containers/theories/IntSetProofs.v
@@ -6892,7 +6892,7 @@ Qed.
 Require Import Coq.FSets.FSetInterface.
 Require Import Coq.Structures.OrderedTypeEx.
 
-Module Foo: WSfun(N_as_OT).
+Module Foo <: WSfun(N_as_OT).
   Module OrdFacts := OrderedTypeFacts(N_as_OT).
 
   (* We are saying [N] instead of [Z] to force the invariant that
