examples/containers/proofs/IntSetProperties.v
@@ -1,0 +1,1 @@
+../lib/intset-properties.v
